src/certigrad/aevb/graph.lean
@@ -15,27 +15,27 @@ namespace aevb
 
 section nodes
 
-open det det.cwise1 det.cwise2 det.special rand.op label tactic certigrad.tactic
+open det rand.op label tactic certigrad.tactic
 
 def graph_naive : Π (a : arch) (x_data : T [a^.n_in, a^.n_x]), graph
 | a x_data :=
-graph.mk [⟨(ID.nat 0, [a^.ne, a^.bs]), [(ID.str W_encode₁, [a^.ne, a^.n_in]), (ID.str x, [a^.n_in, a^.bs])], operator.det $ op.special $ gemm _ _ _⟩,
-          ⟨(ID.nat 1, [a^.ne, a^.bs]), [(ID.nat 0, [a^.ne, a^.bs])], operator.det $ op.unary $ softplus⟩,
-          ⟨(ID.nat 2, [a^.ne, a^.bs]), [(ID.str W_encode₂, [a^.ne, a^.ne]), (ID.nat 1, [a^.ne, a^.bs])], operator.det $ op.special $ gemm _ _ _⟩,
-          ⟨(ID.str h_encode, [a^.ne, a^.bs]), [(ID.nat 2, [a^.ne, a^.bs])], operator.det $ op.unary $ softplus⟩,
-          ⟨(ID.str μ, [a^.nz, a^.bs]), [(ID.str W_encode_μ, [a^.nz, a^.ne]), (ID.str h_encode, [a^.ne, a^.bs])], operator.det $ op.special $ gemm _ _ _⟩,
-          ⟨(ID.nat 5, [a^.nz, a^.bs]), [(ID.str W_encode_logσ₂, [a^.nz, a^.ne]), (ID.str h_encode, [a^.ne, a^.bs])], operator.det $ op.special $ gemm _ _ _⟩,
-          ⟨(ID.nat 6, [a^.nz, a^.bs]), [(ID.nat 5, [a^.nz, a^.bs])], operator.det $ op.unary exp⟩,
-          ⟨(ID.str σ, [a^.nz, a^.bs]), [(ID.nat 6, [a^.nz, a^.bs])], operator.det $ op.unary sqrt⟩,
+graph.mk [⟨(ID.nat 0, [a^.ne, a^.bs]), [(ID.str W_encode₁, [a^.ne, a^.n_in]), (ID.str x, [a^.n_in, a^.bs])], operator.det $ ops.gemm _ _ _⟩,
+          ⟨(ID.nat 1, [a^.ne, a^.bs]), [(ID.nat 0, [a^.ne, a^.bs])], operator.det $ ops.softplus _⟩,
+          ⟨(ID.nat 2, [a^.ne, a^.bs]), [(ID.str W_encode₂, [a^.ne, a^.ne]), (ID.nat 1, [a^.ne, a^.bs])], operator.det $ ops.gemm _ _ _⟩,
+          ⟨(ID.str h_encode, [a^.ne, a^.bs]), [(ID.nat 2, [a^.ne, a^.bs])], operator.det $ ops.softplus _⟩,
+          ⟨(ID.str μ, [a^.nz, a^.bs]), [(ID.str W_encode_μ, [a^.nz, a^.ne]), (ID.str h_encode, [a^.ne, a^.bs])], operator.det $ ops.gemm _ _ _⟩,
+          ⟨(ID.nat 5, [a^.nz, a^.bs]), [(ID.str W_encode_logσ₂, [a^.nz, a^.ne]), (ID.str h_encode, [a^.ne, a^.bs])], operator.det $ ops.gemm _ _ _⟩,
+          ⟨(ID.nat 6, [a^.nz, a^.bs]), [(ID.nat 5, [a^.nz, a^.bs])], operator.det $ ops.exp _⟩,
+          ⟨(ID.str σ, [a^.nz, a^.bs]), [(ID.nat 6, [a^.nz, a^.bs])], operator.det $ ops.sqrt _⟩,
           ⟨(ID.str z, [a^.nz, a^.bs]), [(ID.str μ, [a^.nz, a^.bs]), (ID.str σ, [a^.nz, a^.bs])], operator.rand $ mvn_iso _⟩,
           ⟨(ID.str encoding_loss, []), [(ID.str μ, [a^.nz, a^.bs]), (ID.str σ, [a^.nz, a^.bs]), (ID.str z, [a^.nz, a^.bs])], operator.det $ op.mvn_iso_empirical_kl _⟩,
-          ⟨(ID.nat 10, [a^.nd, a^.bs]), [(ID.str W_decode₁, [a^.nd, a^.nz]), (ID.str z, [a^.nz, a^.bs])], operator.det $ op.special $ gemm _ _ _⟩,
-          ⟨(ID.nat 11, [a^.nd, a^.bs]), [(ID.nat 10, [a^.nd, a^.bs])], operator.det $ op.unary $ softplus⟩,
-          ⟨(ID.nat 12, [a^.nd, a^.bs]), [(ID.str W_decode₂, [a^.nd, a^.nd]), (ID.nat 11, [a^.nd, a^.bs])], operator.det $ op.special $ gemm _ _ _⟩,
-          ⟨(ID.str h_decode, [a^.nd, a^.bs]), [(ID.nat 12, [a^.nd, a^.bs])], operator.det $ op.unary $ softplus⟩,
-          ⟨(ID.nat 14, [a^.n_in, a^.bs]), [(ID.str W_decode_p, [a^.n_in, a^.nd]), (ID.str h_decode, [a^.nd, a^.bs])], operator.det $ op.special $ gemm _ _ _⟩,
-          ⟨(ID.str p, [a^.n_in, a^.bs]), [(ID.nat 14, [a^.n_in, a^.bs])], operator.det $ op.unary $ sigmoid⟩,
-          ⟨(ID.str decoding_loss, []), [(ID.str p, [a^.n_in, a^.bs]), (ID.str x, [a^.n_in, a^.bs])], operator.det $ op.special $ bernoulli_neglogpdf _⟩]
+          ⟨(ID.nat 10, [a^.nd, a^.bs]), [(ID.str W_decode₁, [a^.nd, a^.nz]), (ID.str z, [a^.nz, a^.bs])], operator.det $ ops.gemm _ _ _⟩,
+          ⟨(ID.nat 11, [a^.nd, a^.bs]), [(ID.nat 10, [a^.nd, a^.bs])], operator.det $ ops.softplus _⟩,
+          ⟨(ID.nat 12, [a^.nd, a^.bs]), [(ID.str W_decode₂, [a^.nd, a^.nd]), (ID.nat 11, [a^.nd, a^.bs])], operator.det $ ops.gemm _ _ _⟩,
+          ⟨(ID.str h_decode, [a^.nd, a^.bs]), [(ID.nat 12, [a^.nd, a^.bs])], operator.det $ ops.softplus _⟩,
+          ⟨(ID.nat 14, [a^.n_in, a^.bs]), [(ID.str W_decode_p, [a^.n_in, a^.nd]), (ID.str h_decode, [a^.nd, a^.bs])], operator.det $ ops.gemm _ _ _⟩,
+          ⟨(ID.str p, [a^.n_in, a^.bs]), [(ID.nat 14, [a^.n_in, a^.bs])], operator.det $ ops.sigmoid _⟩,
+          ⟨(ID.str decoding_loss, []), [(ID.str p, [a^.n_in, a^.bs]), (ID.str x, [a^.n_in, a^.bs])], operator.det $ ops.bernoulli_neglogpdf _⟩]
          [ID.str encoding_loss, ID.str decoding_loss]
          [(ID.str W_encode₁, [a^.ne, a^.n_in]), (ID.str W_encode₂, [a^.ne, a^.ne]), (ID.str W_encode_μ, [a^.nz, a^.ne]), (ID.str W_encode_logσ₂, [a^.nz, a^.ne]),
           (ID.str W_decode₁, [a^.nd, a^.nz]), (ID.str W_decode₂, [a^.nd, a^.nd]), (ID.str W_decode_p, [a^.n_in, a^.nd])]
